<head>
  <title>Year 9 Calculus EXT</title>
  <script type="text/javascript"
  src="http://cdn.mathjax.org/mathjax/latest/MathJax.js?config=TeX-AMS-MML_HTMLorMML"></script>
</head>

# Year 9 Calculus

## Please note this is extension and not required for any tests in Year 9

### Straight Lines

![Straight Line](/the-merchant/assets/images/Year%209/Math/straight-line-gradients.jpg)

$\frac{Δy}{Δ}$, where Δ is *change in*.


### Quadratics

![Quadratics](/the-merchant/assets/images/Year%209/Math/quadratics.svg)

$y={x^2}$ or $\frac{dy}{dx}$, where d is *difference in*


### Cubic Equations

![Cubic](/the-merchant/assets/images/Year%209/Math/cubic.png)

To find the gradient, find two points and find the rise/run of those two points for a rough estimate. The closer the points, the better the estimate.  
If we use the function $y=f(x)$, we see that the coordinates of any point would be $(x, f(x))$.  
Supposing that h is the change in x, we can write this as:
$\frac{f(x+h)-f(x)}{h}$.

Therefore, the gradient would be found using

$\lim_{h \to 0} \frac{f(x+h)-f(x)}{h}$.

Example: $f(x) = {x^2}$

$\lim_{h \to 0} (\frac{(x+h)^2 - x^2}{h})$ = $\lim_(h \to 0) (\frac{x^2 + 2xh + h^2 - x^2}{h})$

$\lim_{h \to 0} (\frac{(x+h)^2 - x^2}{h})$ = $\lim_(h \to 0) (\frac{2xh + h^2}{h})$

$\lim_{h \to 0} (\frac{(x+h)^2 - x^2}{h})$ = $\lim_(h \to 0) (\frac{2xh + h}{1})$

$\lim_{h \to 0} (\frac{(x+h)^2 - x^2}{h})$ = $\lim_(h \to 0) (2x+h)$